\documentclass[12pt,letterpaper]{article}
\usepackage[utf8]{inputenc}
\usepackage{amsmath}
\usepackage{amsfonts}
\usepackage{amssymb}
\begin{document}

With only Work done by Gravity

$$\Sigma W = W_g = \Delta K$$

$$W_g = \int_{A}^{B} F_{g} ds$$

$$W_g = \int_{A}^{B} -mg ds$$

$$W_g = -mgs_B + mgs_A$$

$$W_g = mgs_A - mgs_B$$

$$mgs_A - mgs_B = \Delta K$$

$$mgs_A - mgs_B = \frac{1}{2}mv_B^2 - \frac{1}{2}mv_A^2$$

$$mgs_A + \frac{1}{2}mv_A^2  = mgs_B + \frac{1}{2}mv_B^2 $$

Define $U_g = mgs$

$$U_{g, A} + K_A = U_{g, B} + K_B$$

\pagebreak

With only Work done by Spring

$$\Sigma W = W_e = \Delta K$$

$$W_e = \int_{A}^{B} F_e dx$$

$$W_e = \int_{A}^{B} -kx dx$$

$$W_e = -\frac{1}{2}kx_B^2  + \frac{1}{2}kx_A^2$$

$$W_e =  \frac{1}{2}kx_A^2 - \frac{1}{2}kx_B^2$$


$$\frac{1}{2}kx_A^2 - \frac{1}{2}kx_B^2 = \Delta K$$

$$\frac{1}{2}kx_A^2 - \frac{1}{2}kx_B^2 = \frac{1}{2}mv_B^2 - \frac{1}{2}mv_A^2$$

$$\frac{1}{2}kx_A^2  + \frac{1}{2}mv_A^2 = \frac{1}{2}kx_B^2 + \frac{1}{2}mv_B^2$$

Define $U_e = \frac{1}{2}kx^2$

$$U_{e, A} + K_A = U_{e, B} + K_B$$

\pagebreak

With arbitrary conservative force $F_C$

$$\Sigma W = W_C = \Delta K$$

$$W_C = \int_{A}^{B} F_C ds$$

By definition of Conservative Force, There exists a function $f(s)$ where

$$W_C = f(s_B) - f(s_A)$$

Define $W_C = -\Delta U_C$

$$f(s_B) - f(s_A) =  -\Delta U_C$$

$$f(s_B) - f(s_A) = \frac{1}{2}mv_B^2 - \frac{1}{2}mv_A^2$$

$$-\Delta U_C = \frac{1}{2}mv_B^2 - \frac{1}{2}mv_A^2$$

$$-(U_{C,B} - U_{C,A }) = \frac{1}{2}mv_B^2 - \frac{1}{2}mv_A^2$$

$$-U_{C,B} + U_{C,A } = \frac{1}{2}mv_B^2 - \frac{1}{2}mv_A^2$$

$$U_{C,A } + \frac{1}{2}mv_A^2 = U_{C,B} + \frac{1}{2}mv_B^2$$

\pagebreak

\end{document}