\documentclass[12pt,letterpaper]{article}
\usepackage[utf8]{inputenc}
\usepackage{amsmath}
\usepackage{amsfonts}
\usepackage{amssymb}
\begin{document}

\textbf{Uniform Circular Motion Proof} \\

$$\vec{s}(t) = \begin{bmatrix} r\cos(\omega t) \\ r\sin(\omega t) \end{bmatrix}$$ 

$$\vec{v}(t) = \begin{bmatrix} -r\omega \sin (\omega t) \\ r \omega \cos(\omega t) \end{bmatrix}$$ 

$$\vec{a}(t) = \begin{bmatrix} -r\omega^2 \cos (\omega t) \\ -r \omega^2 \sin(\omega t) \end{bmatrix}$$ 

$$|\vec{v}(t)| = \sqrt{(-r\omega \sin (\omega t))^2 + (r \omega \cos(\omega t))^2}$$

$$|\vec{v}(t)| = \sqrt{r^2\omega^2 \sin^2(\omega t) + r^2 \omega^2 \cos^2(\omega t)}$$ 

$$|\vec{v}(t)| = r\omega \sqrt{\sin^2(\omega t) + \cos^2(\omega t)}$$

$$|\vec{v}(t)| = r\omega \sqrt{1}$$

$$|\vec{v}(t)| =  \omega r$$

$$|\vec{a}(t)| = \sqrt{( -r\omega^2 \cos (\omega t))^2 + (-r \omega^2 \sin(\omega t))^2}$$

$$|\vec{a}(t)| = \sqrt{r^2 \omega^4 \cos^2(\omega t) + r^2 \omega^4 \sin^2(\omega t)}$$

$$|\vec{a}(t)| = r \omega ^2 \sqrt{\cos^2(\omega t) + \sin^2(\omega t)}$$

$$|\vec{a}(t)| = r \omega ^2 \sqrt{1}$$

$$|\vec{a}(t)| = \omega ^2 r$$

$$|\vec{a}(t)| = \dfrac{(\omega r)^2}{r}$$

$$|\vec{a}(t)| = \dfrac{|\vec{v}(t)|^2}{r}$$

\textbf{More Stuff}

$$\theta = \omega t$$

$$\dfrac{d\theta}{dt}  = \omega$$

\end{document}