\documentclass[12pt,letterpaper]{article}
\usepackage[utf8]{inputenc}
\usepackage{amsmath}
\usepackage{amsfonts}
\usepackage{amssymb}
\begin{document}

Proof of Work-Energy Theorem

$$ \Sigma W_{AB} = \int_{A}^{B} \Sigma \vec{F}  \cdot d\vec{s}$$

$$ \Sigma W_{AB} = \int_{A}^{B} (\Sigma \vec{F}_x \hat{i} + \Sigma \vec{F}_y \hat{j} + \Sigma \vec{F}_z \hat{k})  \cdot (d\vec{s}_x \hat{i} + d\vec{s}_y \hat{j} + d\vec{s}_z \hat{k})$$

$$ \Sigma W_{AB} = \int_{A}^{B} \Sigma \vec{F}_x d\vec{s}_x  + \Sigma \vec{F}_y d\vec{s}_y + \Sigma \vec{F}_z d\vec{s}_z$$

$$ \Sigma W_{AB} = \int_{A}^{B} \Sigma \vec{F}_x d\vec{s}_x + \int_{A}^{B} \Sigma \vec{F}_y d\vec{s}_y + \int_{A}^{B} \Sigma \vec{F}_z d\vec{s}_z $$

$$\Sigma \vec{F}_x = m\vec{a}_x $$

$$\vec{a}_x = \dfrac{d\vec{v}_x}{dt} $$

$$d\vec{s}_x = \vec{v}_x dt $$

$$\Sigma \vec{F}_x d\vec{s}_x =  m\vec{a}_x  \vec{v}_x dt $$

$$\Sigma \vec{F}_x d\vec{s}_x = m \dfrac{d\vec{v}_x}{dt}  \vec{v}_x dt $$

$$\Sigma \vec{F}_x d\vec{s}_x = m  \vec{v}_x  d\vec{v}_x $$


$$ \Sigma W_{AB} = \int_{A}^{B} m  \vec{v}_x  d\vec{v}_x + \int_{A}^{B} m  \vec{v}_y  d\vec{v}_y + \int_{A}^{B} m  \vec{v}_z  d\vec{v}_z $$

$$ \Sigma W_{AB} = \left .  \frac{1}{2}m\vec{v}_x^2 \right|_{A}^{B} + \left .  \frac{1}{2}m\vec{v}_y^2 \right|_{A}^{B} + \left .  \frac{1}{2}m\vec{v}_z^2 \right|_{A}^{B}$$

$$K_x = \frac{1}{2}m\vec{v}_x^2$$

$$ \Sigma W_{AB} = \Delta K_x + \Delta K_y + \Delta K_z$$

$$ \Sigma W_{AB} = \Delta K$$

\end{document}